.

theories/Logic/ExtraFol.v
@@ -6,6 +6,111 @@ Require Import PnV.Logic.BasicFol.
 Require Import PnV.Logic.BasicFol2.
 Require Import PnV.Logic.HilbertFol.
 
+Section SCOPED.
+
+Context {L : language}.
+
+Definition scoped_trm (xs : list ivar) : Set :=
+  { t : trm L | forall z, is_free_in_trm z t = true -> In z xs }.
+
+Definition scoped_trms (n : nat) (xs : list ivar) : Set :=
+  { ts : trms L n | forall z, is_free_in_trms z ts = true -> In z xs }.
+
+Definition scoped_frm (xs : list ivar) : Set :=
+  { p : frm L | forall z, is_free_in_frm z p = true -> In z xs }.
+
+#[program]
+Definition sRel {xs : list ivar} (R : L.(relation_symbols)) (ts : scoped_trms (L.(relation_arity_table) R) xs) : scoped_frm xs :=
+  @exist _ _ (Rel_frm R (proj1_sig ts)) (fun z : ivar => fun H => _).
+Next Obligation.
+  exact (proj2_sig ts z H).
+Qed.
+
+#[program]
+Definition sEqn {xs : list ivar} (t1 : scoped_trm xs) (t2 : scoped_trm xs) : scoped_frm xs :=
+  @exist _ _ (Eqn_frm t1 t2) (fun z : ivar => fun H => _).
+Next Obligation.
+  rewrite orb_true_iff in H. destruct H as [H | H].
+  - eapply (proj2_sig t1 z H).
+  - eapply (proj2_sig t2 z H).
+Qed.
+
+#[program]
+Definition sNeg {xs : list ivar} (s1 : scoped_frm xs) : scoped_frm xs :=
+  @exist _ _ (Neg_frm (proj1_sig s1)) (fun z : ivar => fun H => _).
+Next Obligation.
+  exact (proj2_sig s1 z H).
+Qed.
+
+#[program]
+Definition sImp {xs : list ivar} (s1 : scoped_frm xs) (s2 : scoped_frm xs) : scoped_frm xs :=
+  @exist _ _ (Imp_frm (proj1_sig s1) (proj1_sig s2)) (fun z : ivar => fun H => _).
+Next Obligation.
+  rewrite orb_true_iff in H. destruct H as [H | H].
+  - eapply (proj2_sig s1 z H).
+  - eapply (proj2_sig s2 z H).
+Qed.
+
+#[program]
+Definition sAll {xs : list ivar} (y : ivar) (s1 : scoped_frm (y :: xs)) : scoped_frm xs :=
+  @exist _ _ (All_frm y (proj1_sig s1)) (fun z : ivar => fun H => _).
+Next Obligation.
+  s!. destruct H as [FREE NE]. pose proof (proj2_sig s1 z FREE) as claim. simpl in claim.
+  destruct claim as [EQ | IN]; [now contradiction NE | exact IN].
+Qed.
+
+#[program]
+Definition Con_trm_nil_scoped (c : L.(constant_symbols)) : scoped_trm [] :=
+  @exist _ _ (Con_trm c) _.
+
+#[program]
+Definition subst_one_frm_nil_scoped (y : ivar) (t : scoped_trm []) (p : scoped_frm [y]) : scoped_frm [] :=
+  @exist _ _ (subst_frm (one_subst y (proj1_sig t)) (proj1_sig p)) _.
+Next Obligation.
+  revert z H.
+  assert (claim1 : forall z : ivar, is_free_in_frm z (proj1_sig p) = true -> z = y).
+  { intros z FREE. now pose proof (proj2_sig p z FREE) as [EQ | []]. }
+  assert (claim2 : forall z : ivar, is_not_free_in_trm z (proj1_sig t)).
+  { intros z. red. pose proof (proj2_sig t z). destruct (is_free_in_trm z (proj1_sig t)) as [ | ]; [now contradiction H | reflexivity]. }
+  intros z H. pose proof (one_fv_frm_subst_closed_term_close_formula y (proj1_sig t) (proj1_sig p) claim1 claim2 z) as claim3. red in claim3.
+  enough (WTS : true = false) by discriminate. rewrite <- H. rewrite <- claim3. reflexivity.
+Qed.
+
+Lemma closed_frm_is_sentence (p : frm L)
+  : L.null (fvs_frm (closed_frm p)) = true.
+Proof.
+  rewrite L.null_spec. destruct (fvs_frm (closed_frm p)) as [ | z zs] eqn: H_OBS; trivial.
+  contradiction (closed_frm_closed p z). rewrite <- fv_is_free_in_frm. rewrite H_OBS; simpl; left; trivial.
+Qed.
+
+Definition sentence : Set :=
+  { p : frm L | L.null (fvs_frm p) = true }.
+
+#[program]
+Definition sentence_isEnumerable (enum_frm_L : isEnumerable (frm L)) : isEnumerable sentence :=
+  {| enum n := @exist _ _ (closed_frm (enum n)) (closed_frm_is_sentence (enum n)) |}.
+Next Obligation.
+  unfold closed_frm. destruct x as [p p_eq]; simpl in *.
+  assert (EQ : (close_ivars p (nodup eq_dec (fvs_frm p))) = p). 
+  { enough (WTS : (nodup eq_dec (fvs_frm p)) = []) by now rewrite WTS.
+    destruct (nodup eq_dec (fvs_frm p)) as [ | z zs] eqn: H_OBS.
+    - reflexivity.
+    - assert (claim : L.In z (fvs_frm p)).
+      { rewrite <- L.nodup_In with (decA := eq_dec). rewrite H_OBS. simpl. left. reflexivity. }
+      rewrite L.null_spec in p_eq. rewrite p_eq in claim. contradiction claim.
+  }
+  exists (proj1_sig (enum_spec p)). destruct (enum_spec p) as [n n_eq]; simpl.
+  rewrite <- n_eq in EQ. rewrite @exist_eq_bool with (A := frm L) (P := fun p => L.null (fvs_frm p)).
+  rewrite EQ. exact n_eq.
+Qed.
+
+End SCOPED.
+
+#[global] Arguments scoped_trm : clear implicits.
+#[global] Arguments scoped_trms : clear implicits.
+#[global] Arguments scoped_frm : clear implicits.
+#[global] Arguments sentence : clear implicits.
+
 Module ND.
 
 Section NATURAL_DEDUCTION.
